Got recursive AndN working.

Attempt2/Build/And.dfy
@@ -15,228 +15,25 @@ module Build.AndBuilder {
   {
   }
 
-  function AndSF(n: nat, si: SI): (so: SO)
+  function AndSF(si: SI): (so: SO)
     requires |si.inputs| == 2
     requires |si.state| == 0
   {
     SO([si.inputs[0] && si.inputs[1]], [])
   }
 
-  //trait {:termination false} Model<Inputs, Outputs, State> {
-  //  function Behav(inputs: Inputs, state: State): (r: (Outputs, State))
-  //  function SC(): set<CNode>
-  //  function InputsToMap(inputs: Inputs): (mapped: map<NP, bool>)
-  //    ensures mapped.Keys == Inputs()
-  //  function OutputsToMap(outputs: Outputs): (mapped: map<NP, bool>)
-  //    ensures mapped.Keys == Outputs()
-  //  function OldStateToMap(state: State): (mapped: map<NP, bool>)
-  //    ensures mapped.Keys == StateONPs(State())
-  //  function NewStateToMap(state: State): (mapped: map<NP, bool>)
-  //    ensures mapped.Keys == StateINPs(State())
-  //  function MapToInputs(mapped: map<NP, bool>): (inputs: Inputs)
-  //    requires mapped.Keys == Inputs()
-  //  function MapToOutputs(mapped: map<NP, bool>): (outputs: Outputs)
-  //    requires mapped.Keys == Outputs()
-  //  function MapToNewState(mapped: map<NP, bool>): (state: State)
-  //    requires mapped.Keys == StateINPs(State())
-  //  function MapToOldState(mapped: map<NP, bool>): (state: State)
-  //    requires mapped.Keys == StateONPs(State())
-  //  predicate UniqueElements()
-  //  function Inputs(): set<NP>
-  //  function Outputs(): set<NP>
-  //  function State(): set<CNode>
-  //  function OldStateNPs(): set<NP>
-  //  {
-  //    StateONPs(State())
-  //  }
-  //  function NewStateNPs(): set<NP>
-  //  {
-  //    StateINPs(State())
-  //  }
-  //  function MapBehav(fi: FI): (fo: FO)
-  //    requires FIValid(fi, Inputs(), State())
-  //    ensures FOValid(fo, Outputs(), State())
-  //  {
-  //    var inputs := MapToInputs(fi.inputs);
-  //    var state := MapToOldState(fi.state);
-  //    var (outputs, new_state) := Behav(inputs, state);
-  //    var outputs_map := OutputsToMap(outputs);
-  //    var state_map := NewStateToMap(new_state);
-  //    FO(outputs_map, state_map)
-  //  }
-  //  function MF(): MapFunction
-  //  {
-  //    MapFunction(
-  //      Inputs(), Outputs(), State(),
-  //      (fi: FI) requires FIValid(fi, Inputs(), State()) => MapBehav(fi)
-  //    )
-  //  }
-  //  function E(): Entity
-  //  {
-  //    Entity(SC(), MF())
-  //  }
-  //}
-
-  //// A generic trait used to bundle some constants, functions and lemmas together.
-  //trait {:termination false} Flattenable<T> {
-
-  //  // I don't want to specify the value of length here.
-  //  const length: nat := 2
-
-  //  function tobits(a: T): (r: seq<bool>)
-  //    ensures |r| == length
-  //  function frombits(bs: seq<bool>): (r: T)
-  //    requires |bs| == length
-  //  lemma flattenable(a: T)
-  //    ensures frombits(tobits(a)) == a
-  //}
-
-  //// An example datatype that I want to be able to apply these functions and lemmas to.
-  //datatype AndInputs = AndInputs(
-  //  i_0: bool,
-  //  i_1: bool
-  //  )
-
-  //// An implementation of these functions and lemmas for this type.
-  //datatype FlattenableAndInputs extends Flattenable<AndInputs> = FlattenableAndInputs() {
-
-  //  // I want to specify the value of length here.
-  //  //const length: nat := 2
-
-  //  function tobits(a: AndInputs): (r: seq<bool>)
-  //    ensures |r| == length
-  //  {
-  //    [a.i_0, a.i_1]
-  //  }
-
-  //  function frombits(bs: seq<bool>): (r: AndInputs)
-  //    requires |bs| == length
-  //  {
-  //    AndInputs(bs[0], bs[1])
-  //  }
-
-  //  lemma flattenable(a: AndInputs)
-  //    ensures frombits(tobits(a)) == a
-  //  {
-  //    var bs := tobits(a);
-  //    assert |bs| == length;
-  //    assert frombits(bs) == a;
-  //  }
-  //}
-
-  //// Some example uses where the bundle of functions and lemmas can be used for
-  //// any type. The specifc implementations are passed in as f.
-
-  //function ExampleFlattener<X>(x: X, f: Flattenable<X>): seq<bool>
-  //{
-  //  f.tobits(x)
-  //}
-
-  //function ExampleUnflattener<X>(b: seq<bool>, f: Flattenable<X>): X
-  //  requires |b| == f.length
-  //{
-  //  f.frombits(b)
-  //}
-
-  //lemma ExampleCorrect<X>(x: X, f: Flattenable<X>)
-  //  ensures f.frombits(f.tobits(x)) == x
-  //{
-  //  f.flattenable(x);
-  //}
-
-  //datatype AndOutputs = AndOutputs(
-  //  o: bool
-  //  )
-
-  //datatype AndState = AndState()
-
-  //datatype AndInputMapping = AndInputMapping(
-  //  i_0: NP,
-  //  i_1: NP
-  //  )
-
-  //datatype AndOutputMapping = AndOutputMapping(
-  //  o: NP
-  //  )
-
-  //datatype AndStateMapping = AndStateMapping()
-
-  //function AndBehav(inputs: AndInputs, state: AndState): (r: (AndOutputs, AndState))
-  //{
-  //  (AndOutputs(inputs.i_0 && inputs.i_1), AndState())
-  //}
-
-  //datatype And extends Model<AndInputs, AndOutputs, AndState> =
-  //  And(im: AndInputMapping, om: AndOutputMapping, sm: AndStateMapping,
-  //      sc: set<CNode>) {
-  //  function Behav(inputs: AndInputs, state: AndState): (r: (AndOutputs, AndState))
-  //  {
-  //    AndBehav(inputs, state)
-  //  }
-  //  function SC(): set<CNode> { sc }
-  //  function InputsToMap(inputs: AndInputs): (mapped: map<NP, bool>)
-  //    ensures mapped.Keys == Inputs()
-  //  {
-  //    map[im.i_0 := inputs.i_0, im.i_1 := inputs.i_1]
-  //  }
-  //  function OutputsToMap(outputs: AndOutputs): (mapped: map<NP, bool>)
-  //    ensures mapped.Keys == Outputs()
-  //  {
-  //    map[om.o := outputs.o]
-  //  }
-  //  function OldStateToMap(state: AndState): (mapped: map<NP, bool>)
-  //    ensures mapped.Keys == StateONPs(State())
-  //  {
-  //    map[]
-  //  }
-  //  function NewStateToMap(state: AndState): (mapped: map<NP, bool>)
-  //    ensures mapped.Keys == StateINPs(State())
-  //  {
-  //    map[]
-  //  }
-  //  function MapToInputs(mapped: map<NP, bool>): (inputs: AndInputs)
-  //    requires mapped.Keys == Inputs()
-  //  {
-  //   AndInputs(mapped[im.i_0], mapped[im.i_1])
-  //  }
-  //  function MapToOutputs(mapped: map<NP, bool>): (outputs: AndOutputs)
-  //    requires mapped.Keys == Outputs()
-  //  {
-  //   AndOutputs(mapped[om.o])
-  //  }
-  //  function MapToNewState(mapped: map<NP, bool>): (state: AndState)
-  //    requires mapped.Keys == StateINPs(State())
-  //  {
-  //   AndState()
-  //  }
-  //  function MapToOldState(mapped: map<NP, bool>): (state: AndState)
-  //    requires mapped.Keys == StateONPs(State())
-  //  {
-  //   AndState()
-  //  }
-  //  predicate UniqueElements()
-  //  {
-  //    && im.i_0 != im.i_1
-  //    && im.i_0 != om.o
-  //    && im.i_1 != om.o
-  //  }
-  //  function Inputs(): set<NP>
-  //  {
-  //    {im.i_0, im.i_1}
-  //  }
-  //  function Outputs(): set<NP>
-  //  {
-  //    {om.o}
-  //  }
-  //  function State(): set<CNode>
-  //  {
-  //    {}
-  //  }
-  //  function All(): set<NP>
-  //  {
-  //    Inputs() + Outputs() + StateINPs(State()) + StateONPs(State())
-  //  }
-  //}
+  ghost predicate AndMFValid(mf: MapFunction)
+  {
+    && mf.Valid()
+    && |mf.inputs| == 2
+    && |mf.state| == 0
+    && |mf.outputs| == 1
+    && (forall si :: SIValid(si, mf.inputs, mf.state) ==> (
+      && mf.sf.requires(si)
+      && mf.sf(si) == AndSF(si)
+      )
+    )
+  }
 
   function InsertAndImpl(c: Circuit): (r: (Circuit, Entity))
     requires CircuitValid(c)
